refactor: Untyped

TTFPI/Untyped.lean
@@ -1,7 +1,7 @@
 import TTFPI.Basic
 
 -- 1.3.2: The set Λ of all λ-terms
-@[reducible] def Name := String
+abbrev Name := String
 
 inductive Λ where
 | var : Name → Λ
@@ -12,26 +12,24 @@ deriving Repr, BEq, Ord
 namespace Λ
 
 -- 1.3.5: Multiset of subterms
-@[simp] def Sub (t : Λ) : List Λ :=
+def Sub (t : Λ) : List Λ :=
   match t with
   | var _ => [t]
   | app M N => t :: (Sub M ++ Sub N)
   | abs _ M => t :: Sub M
 
-@[simp] def Subterm (L M : Λ) : Prop := L ∈ Sub M
-
 -- 1.3.6
-theorem reflexivity (M : Λ) : Subterm M M := by
-  cases M <;> simp
+theorem reflexivity (M : Λ) : M ∈ Sub M := by
+  cases M <;> simp [Sub]
 
-theorem transitivity (L M N : Λ) : Subterm L M ∧ Subterm M N → Subterm L N := by
+theorem transitivity (L M N : Λ) : L ∈ Sub M ∧ M ∈ Sub N → L ∈ Sub N := by
   simp
   intros hlm hmn
   induction N with
   | var _ =>
-    simp at *
+    simp [Sub] at *
     rw [hmn] at hlm
-    simp at *
+    simp [Sub] at *
     exact hlm
   | app M N ihlm ihln =>
     sorry
@@ -39,16 +37,16 @@ theorem transitivity (L M N : Λ) : Subterm L M ∧ Subterm M N → Subterm L N 
     sorry
 
 -- 1.3.8: Proper subterm
-def ProperSubterm (L M : Λ) : Prop := Subterm L M ∧ L ≠ M
+def ProperSubterm (L M : Λ) : Prop := L ∈ Sub M ∧ L ≠ M
 
 -- 1.4.1: The set of free variables of a λ-term
-def FreeVariables : Λ → RBSet Λ
+def FV : Λ → RBSet Λ
 | t@(var _) => .single t
-| app M N => FreeVariables M ∪ FreeVariables N
-| abs x M => FreeVariables M \ .single (var x)
+| app M N => FV M ∪ FV N
+| abs x M => FV M \ .single (var x)
 
 -- 1.4.3: Closed λ-term; combinator; Λ⁰
-def Closed (M : Λ) : Prop := FreeVariables M = ∅
+def Closed (M : Λ) : Prop := FV M = ∅
 
 -- 1.5.1: Renaming; Mˣ ʸ; =ₐ
 def rename (x y : Name) : Λ → Λ
@@ -63,10 +61,10 @@ def Renaming (M : Λ) (x y : Name) (N : Λ) : Prop := rename x y M = N
 def ex : Λ := abs "x" (app (var "x") (var "y"))
 
 #eval Sub ex
--- #eval Subterm (var "x") ex
+-- #eval (var "x") ∈ Sub ex
 -- #eval ProperSubterm (var "x") ex
-#eval FreeVariables ex
-#eval FreeVariables $ app (var "x") (abs "x" (app (var "x") (var "y")))
+#eval FV ex
+#eval FV $ app (var "x") (abs "x" (app (var "x") (var "y")))
 -- #eval Closed $ abs "x" (var "x")
 #eval rename "x" "a" ex |> rename "x" "b"
 
